

(1)

Derivation

Eq 1: $S = \begin{pmatrix} 1 & 0 & 0 \\ 0 & 1 & 0 \end{pmatrix} \left[\begin{bmatrix} R \begin{pmatrix} u'_2 \\ v'_2 \\ 1 \end{pmatrix} + d'_2 T \end{bmatrix} - \begin{pmatrix} z_1/z_2 \end{pmatrix} \begin{pmatrix} u'_1 \\ v'_1 \\ 1 \end{pmatrix} \right]$

Eq 2: $S = \begin{pmatrix} 1 & 0 & -u'_1 \\ 0 & 1 & -v'_1 \end{pmatrix} \left[R \begin{pmatrix} u'_2 \\ v'_2 \\ 1 \end{pmatrix} + d'_2 T \right]$

Sol'n

$\Rightarrow z_1/z_2 = (0 \ 0 \ 1) \left[R \begin{pmatrix} u'_2 \\ v'_2 \\ 1 \end{pmatrix} + d'_2 T \right]$

Substitute

$\Rightarrow \begin{pmatrix} 1 & 0 & 0 \\ 0 & 1 & 0 \end{pmatrix} \left[\begin{bmatrix} R \begin{pmatrix} u'_2 \\ v'_2 \\ 1 \end{pmatrix} + d'_2 T \end{bmatrix} - \underbrace{(0 \ 0 \ 1)}_{1 \times 3} \underbrace{\left[R \begin{pmatrix} u'_2 \\ v'_2 \\ 1 \end{pmatrix} + d'_2 T \right]}_{3 \times 1} \begin{pmatrix} u'_1 \\ v'_1 \\ 1 \end{pmatrix} \right]$

$R = \begin{bmatrix} r_{11} & r_{12} & r_{13} \\ r_{21} & r_{22} & r_{23} \\ r_{31} & r_{32} & r_{33} \end{bmatrix}$

$\Rightarrow \begin{pmatrix} r_{11} & r_{12} & r_{13} \\ r_{21} & r_{22} & r_{23} \\ r_{31} & r_{32} & r_{33} \end{pmatrix} \begin{pmatrix} u'_2 \\ v'_2 \\ 1 \end{pmatrix} = \begin{pmatrix} r_{11}u'_2 + r_{12}v'_2 + r_{13} \\ r_{21}u'_2 + r_{22}v'_2 + r_{23} \\ r_{31}u'_2 + r_{32}v'_2 + r_{33} \end{pmatrix} = R \begin{pmatrix} u'_2 \\ v'_2 \\ 1 \end{pmatrix}$

$d'_2 T = d'_2 \begin{pmatrix} t_1 \\ t_2 \\ t_3 \end{pmatrix} = \begin{pmatrix} d'_2 t_1 \\ d'_2 t_2 \\ d'_2 t_3 \end{pmatrix} = d_2 T$

$\Rightarrow R \begin{pmatrix} u'_2 \\ v'_2 \\ 1 \end{pmatrix} + d_2 T = \begin{pmatrix} r_{11}u'_2 + r_{12}v'_2 + r_{13} + d_2 t_1 \\ r_{21}u'_2 + r_{22}v'_2 + r_{23} + d_2 t_2 \\ r_{31}u'_2 + r_{32}v'_2 + r_{33} + d_2 t_3 \end{pmatrix} = d'$

$$\Rightarrow \begin{pmatrix} 0 & 0 & 1 \end{pmatrix} (a')$$

②

$$= \begin{pmatrix} 0 & 0 & 1 \end{pmatrix} \begin{pmatrix} r_{11}u_2' + r_{12}v_2' + r_{13} + d_2't_3 \\ r_{21}u_2' + r_{22}v_2' + r_{23} + d_2't_3 \\ r_{31}u_2' + r_{32}v_2' + r_{33} + d_2't_3 \end{pmatrix}$$

$$= r_{31}u_2' + r_{32}v_2' + r_{33} + d_2't_3 \begin{pmatrix} u_1' \\ v_1' \\ 1 \end{pmatrix}$$

$$= \begin{pmatrix} [r_{31}u_2' + r_{32}v_2' + r_{33} + d_2't_3] u_1' \\ [r_{31}u_2' + r_{32}v_2' + r_{33} + d_2't_3] v_1' \\ [r_{31}u_2' + r_{32}v_2' + r_{33} + d_2't_3] 1 \end{pmatrix} = b$$

$$\Rightarrow \begin{pmatrix} 1 & 0 & 0 \\ 0 & 1 & 0 \end{pmatrix} \left[R \begin{pmatrix} u_2' \\ v_2' \\ 1 \end{pmatrix} + d_2'T \right] = b$$

$$\Rightarrow \begin{pmatrix} 1 & 0 & 0 \\ 0 & 1 & 0 \end{pmatrix} b = r_{31}u_2' + r_{32}v_2' + r_{33} + d_2't_3 \begin{pmatrix} u_1' \\ v_1' \end{pmatrix}$$

$$\begin{pmatrix} 1 & 0 & 0 \\ 0 & 1 & 0 \end{pmatrix} a = \begin{pmatrix} r_{11}u_2' + r_{12}v_2' + r_{13} + d_2't_3 \\ r_{21}u_2' + r_{22}v_2' + r_{23} + d_2't_3 \end{pmatrix}$$

$$\Rightarrow \begin{pmatrix} r_{11}u_2' + r_{12}v_2' + r_{13} + d_2't_3 \\ r_{21}u_2' + r_{22}v_2' + r_{23} + d_2't_3 \end{pmatrix} = \begin{pmatrix} r_{31}u_2' + r_{32}v_2' + r_{33} + d_2't_3 \\ r_{31}u_2' + r_{32}v_2' + r_{33} + d_2't_3 \end{pmatrix}$$

Expanding Eq 2.

3

$$\Rightarrow \begin{pmatrix} 1 & 0 & -u_1 \\ 0 & 1 & -r_1 \end{pmatrix} \begin{bmatrix} r_{11}u_2' + r_{12}v_2' + r_{13} + d_2't_1 \\ r_{21}u_1' + r_{22}v_2' + r_{23} + d_2't_2 \\ r_{31}u_2' + r_{32}v_2' + r_{33} + d_2't_3 \end{bmatrix}$$

$$\Rightarrow \begin{pmatrix} r_{11}u_2' + r_{12}v_2' + r_{13} + d_2't_1 \\ r_{21}u_1' + r_{22}v_2' + r_{23} + d_2't_2 \end{pmatrix} - \begin{pmatrix} r_{31}u_2'u_1' + r_{32}v_2'u_1' + r_{33}u_1' + d_2't_3u_1' \\ r_{31}u_2'v_1' + r_{32}v_2'v_1' + r_{33}v_1' + d_2't_3v_1' \end{pmatrix}$$

The expressions are equivalent, thus the statement is proved.